Ite.v
@@ -25,8 +25,8 @@ Module IteGadget(PF: GaloisField).
 
   (** Example 1: Division *)
   Definition ite :=
-    <{ \_: Field * Field * Field,
-           if to_bool (fst #0) then fst (snd #0) else snd (snd #0)
+    <{ \_: Bool * Field * Field,
+           if fst #0 then fst (snd #0) else snd (snd #0)
      }>. 
 
   Definition ite_check :=
@@ -36,167 +36,23 @@ Module IteGadget(PF: GaloisField).
   Theorem ite_equiv_r1cs:
     ite <=*=> ite_check.
   Proof.
-    unfold ite_check, r1cs_equiv, ite.
+    unfold ite_check, r1cs_lambda_equiv, ite.
     intros.
-    cbn in vars.  
-    unfold vec_to_exp.
-    unfold Vfp in *.
-    (** Need to get inputs: Vector.t Fp 1 => [ p: Fp ] *)
-    pose proof (vec3_proj inputs).
-    pose proof (vec1_proj outputs).
-    exists_inverter.
-    subst.
-    cbn.
-    destruct (FTH).
-    invert F_R.
-    split; intro H.
-    - (** evaluate the r1cs term *)
-      constructor; cbn.
-      ring_simplify.
-      repeat rewrite Rmul_1_l.
-      destruct (eq_field a0 1:%p) eqn:Ea0.
-      + rewrite e.
-        repeat rewrite Rmul_1_l.
-        rewrite <- Ropp_pkmul.
-        
-        rewrite Rsub_def.
-        replace (pkopp (pkopp b)) with b by ring.
-        (** ((c - b) - a) + b *)
-        replace (pkplus (pksub (pkplus c (pkopp b)) a) b) with (pksub c a) by ring.
-        solve_stlc.
+    cbn in vars, inps, outs, HcannonIn, HcannonOut.
+    unfold correct, correct_lt.
+    split; intros HPrem;
+      invert HeT; cbn in H1; pick fresh x for L; specialize (H1 x Fr); invert H1;
+        repeat invert_types; subst;
+          pose proof (vec3_proj inps); exists_inverter; deconj;
+            pose proof (vec1_proj outs); exists_inverter; deconj; subst;
+              pose proof (cannonical_forms_bool_bool args a b HcannonIn) as HcasesIn;
+              pose proof (cannonical_forms_bool result a0 HcannonOut) as HcasesOut;
+              clear HcannonIn HcannonOut.
+    - (** Backwards reasoning *)
+      deconj; econstructor; cbn; try constructor.
+      + now autorewrite with pk using trivial.
         admit.
-        replace (pksub a a) with (0:%p) by ring.
-        reflexivity.
-      + 
-    - cbn in H.
-      invert H.
-      cbn.
-      econstructor.
-      beta.
-      cbn.
-      econstructor.
-      apply step_if_cog; repeat econstructor.
-      app
-      destruct (eq_bool <{ cast fp a0 }>).
-      econstructor.
-      econstructor.
-      
-      apply multi_step with
-          (y:=              
-             <{
-               if cast (<{ fp a0 }>)
-               then <{ fp b }>
-               else <{ fp c }> }>).
-      
-                          econstructor.
-      cbn i
-      beta.
-      
-      beta.
-      
-      beta (Metatheory.add x
-        econstructor.
-        econstructor.
-        econstructor.
-      + repeat econstructor.
-      + econstructor.
-        cbn.
-      solve_stlc.
-      invert H2.
-      rewrite Rmul_1_l.
-      rewrite Rmul_comm.
-      rewrite Finv_l.
-      apply zirr.
-      cbn.
-      rewrite Z.sub_diag.
-      reflexivity.
-
-      apply neq_stlc_fp in H9.
-      exact H9.
-
-      constructor.
-    - (** evaluate the lambda term *)
-      econstructor.
-      apply step_beta; try constructor.
-      apply (lc_tm_abs empty); intros; solve_stlc.
-      cbn.
-      econstructor.
-      (** single step *)
-      apply step_div_const.
-      
-      (** evaluate the r1cs term *)
-      invert Hprem.
-      rename H6 into Hr1cs.
-      do 2 rewrite Rmul_1_l in Hr1cs.
-
-      destruct (eq_field (hd inputs) 0:%p); solve_stlc.
-      + (** hd inputs = 0 *)
-        rewrite e in Hr1cs.
-        rewrite Rmul_comm in Hr1cs.
-        rewrite fp_mul_zero_l in Hr1cs.
-        pose proof pk_sub_wrap.
-        contradiction.
-      + (** hd inputs <> 0 *)
-        intro.
-        invert H3.
-        contradiction.
-      (** big-step *)
-      + invert Hprem.
-        do 2 rewrite Rmul_1_l in H6.
-        
-
- 
-        rewrite Rsub_def in Hr1cs.
-        
-        invert Hr1cs.
-        cbn in H4.
-        apply Z.lt_gt in H1.
-        
-        rewrite Zdiv.Z_mod_zero_opp in H4.
-        
-        
-        apply Zdiv.Z_mod_zero_opp
-
-        
-
-
-
-        rewrite H1 in H2.
-        apply H in H2.
-        
-        cbn in H2.
-        rewrite H1 in H2.
-        inversion H2.
-        destruct (p_prime).
-        apply Z.lt_gt in H6.        
-        apply gt_relax.
-        exact H6.
-      + (** hd inputs = Z.pos z *)
-        admit.
-      + admit.
-
-        Unshelve.
-        exact empty.
-        
-        rewrite H1 in H2.
-      apply multi_refl.
-      rewrite Fdiv_def in Hr1cs.
-      
-      econstructor; solve_stlc.
-      solve_stlc.
-      Search Z.sub.
-      Search modulo.
-      cbn.
-      destruct p.
-      Print inv.
-      rewrite Z.mul_assoc.
-      simple inversion Hlambda.
-      rewrite H in H0.
-      remember (pkmul 1 :%p (pkinv {| val := inp; inZnZ := inZnZ |})) as out_inv.
-      remember ({| val := out; inZnZ := inZnZ0 |}) as out_fp.
-      
-      unfold pK in out_inv.
-      
+    - (** Forward reasoning *)
   Admitted.
 
 End IteGadget.     
